src/test/output/adjList.dfy
@@ -1,24 +1,34 @@
-datatype List<T> = Nil | Cons(head :T, tail :List<T>)
-function validAdjListM(adjList :seq<List<int>>, N :int, pos :int): bool
+datatype List<T> = Nil | Cons(head: T, tail: List<T>)
+
+function validAdjListM(adjList: seq<List<int>>, N: int, pos: int): bool
 requires (N >= 1 && pos >= 0 && pos <= N && N == |adjList|)
 decreases (pos)
-{if pos == 0 then true else validListM(adjList[pos - 1], N) && validAdjListM(adjList, N, pos - 1)}function validAdjList(adjList :seq<List<int>>, N :int, pos :int): bool
+{if pos == 0 then true else validListM(adjList[pos - 1], N) && validAdjListM(adjList, N, pos - 1)}
+
+function validAdjList(adjList: seq<List<int>>, N: int, pos: int): bool
 requires (N >= 1 && pos >= 0 && pos <= N && N == |adjList|)
 decreases (pos)
-{if (pos == 0) then true else if (validAdjList(adjList, N, pos - 1)) then validList(N, adjList[pos - 1]) else false}function validList(N :int, l :List<int>): bool
+{if (pos == 0) then true else if (validAdjList(adjList, N, pos - 1)) then validList(N, adjList[pos - 1]) else false}
+
+function validList(N: int, l: List<int>): bool
 requires (N >= 1)
 {match l {
 case Cons(h, t) => if (h >= 0 && h < N) then validList(N, t) else false
 case Nil => true
 }
-}function validListM(list :List<int>, N :int): bool
+}
+
+function validListM(list: List<int>, N: int): bool
 requires (N >= 1)
 {match list {
 case Nil() => true
 case Cons(h, t) => h >= 0 && h < N && validListM(t, N)
 }
-}lemma validAdjListEquivalence(adjList :seq<List<int>>, N :int, pos :int)
+}
+
+lemma validAdjListEquivalence(adjList: seq<List<int>>, N: int, pos: int)
 requires (N >= 1 && pos >= 0 && pos <= N && N == |adjList|)
 decreases (pos)
 ensures validAdjListM(adjList, N, pos) == validAdjList(adjList, N, pos)
 {{}}
+
