src/test/output/arrayIncreasing.dfy
@@ -1,12 +1,19 @@
-function validLengthIncreasingM(a :seq<seq<int>>, N :int, M :int, k :int): bool
+function validLengthIncreasingM(a: seq<seq<int>>, N: int, M: int, k: int): bool
 requires (N > 0 && N == |a| && M > 0 && k >= 0 && k <= N)
 decreases (N - k)
-{if (k == N) then true else |a[k]| == M && validLengthIncreasingM(a, N, M, succM(k))}function validLengthIncreasing(a :seq<seq<int>>, N :int, M :int, k :int): bool
+{if (k == N) then true else |a[k]| == M && validLengthIncreasingM(a, N, M, succM(k))}
+
+function validLengthIncreasing(a: seq<seq<int>>, N: int, M: int, k: int): bool
 requires (N > 0 && N == |a| && M > 0 && k >= 0 && k <= N)
 decreases (N - k)
-{if (k == N) then true else |a[k]| == M && validLengthIncreasing(a, N, M, k + 1)}function succM(n :int): int
-{n + 1}lemma validLengthIncreasingEquivalence(a :seq<seq<int>>, N :int, M :int, k :int)
+{if (k == N) then true else |a[k]| == M && validLengthIncreasing(a, N, M, k + 1)}
+
+function succM(n: int): int
+{n + 1}
+
+lemma validLengthIncreasingEquivalence(a: seq<seq<int>>, N: int, M: int, k: int)
 requires (N > 0 && N == |a| && M > 0 && k >= 0 && k <= N)
 decreases (N - k)
 ensures validLengthIncreasingM(a, N, M, k) == validLengthIncreasing(a, N, M, k)
 {{}}
+
