src/test/output/factorial.dfy
@@ -1,5 +1,10 @@
-function fact14_1(n :int): int
-{if (n <= 1) then 1 else n * fact14_1(n - 1)}function fact14_2(n :int): int
-{if (n <= 1) then 1 else if (n == 10) then 3628800 else n * fact14_2(n - 1)}lemma fact14_2Equivalence(n :int)
+function fact14_1(n: int): int
+{if (n <= 1) then 1 else n * fact14_1(n - 1)}
+
+function fact14_2(n: int): int
+{if (n <= 1) then 1 else if (n == 10) then 3628800 else n * fact14_2(n - 1)}
+
+lemma fact14_2Equivalence(n: int)
 ensures fact14_1(n) == fact14_2(n)
 {{}}
+
