src/test/output/foolproof.dfy
@@ -1,23 +1,33 @@
-datatype List<T> = Nil | Cons(head :T, tail :List<T>)
-function funnyZipM(xs :List<int>, ys :List<int>): List<int>
+datatype List<T> = Nil | Cons(head: T, tail: List<T>)
+
+function funnyZipM(xs: List<int>, ys: List<int>): List<int>
 decreases (xs)
 {match (xs, ys) {
 case (_, Nil) => Nil
 case (Nil, _) => Nil
 case (Cons(x, xs), Cons(y, ys)) => Cons(chooseM(x, y), funnyZipM(xs, ys))
 }
-}function funnyZip1(xs :List<int>, ys :List<int>): List<int>
+}
+
+function funnyZip1(xs: List<int>, ys: List<int>): List<int>
 decreases (xs)
 {match (xs, ys) {
 case (_, Nil) => Nil
 case (Nil, _) => Nil
 case (Cons(x, xs), Cons(y, ys)) => Cons(choose1(x, y), funnyZip1(xs, ys))
 }
-}function choose1(x :int, y :int): int
+}
+
+function choose1(x: int, y: int): int
 decreases (if (x <= 0) then 0 else x)
-{if (x <= 0) then y else if (y <= 0) then x else choose1(x - 1, y - 1)}function chooseM(x :int, y :int): int
+{if (x <= 0) then y else if (y <= 0) then x else choose1(x - 1, y - 1)}
+
+function chooseM(x: int, y: int): int
 decreases (if (x <= 0) then 0 else x)
-{if (x <= 0) then y else if (y <= 0) then x else chooseM(x - 1, y - 1)}lemma funnyZip1Equivalence(xs :List<int>, ys :List<int>)
+{if (x <= 0) then y else if (y <= 0) then x else chooseM(x - 1, y - 1)}
+
+lemma funnyZip1Equivalence(xs: List<int>, ys: List<int>)
 decreases (xs)
 ensures funnyZipM(xs, ys) == funnyZip1(xs, ys)
 {{}}
+
