src/test/output/funnyarith2.dfy
@@ -1,28 +1,46 @@
 datatype OpKind = Add | Sub | Mul
-function evalM(op :OpKind, x :int, y :int): int
+
+function evalM(op: OpKind, x: int, y: int): int
 {match op {
 case Add => add(x, y)
 case Sub => sub(x, y)
 case Mul => mul(x, y)
 }
-}function eval1(op :OpKind, x :int, y :int): int
+}
+
+function eval1(op: OpKind, x: int, y: int): int
 {match op {
 case Sub => mySub(y, x)
 case Mul => myMul(x, y)
 case Add => myAdd(x, y)
 }
-}function myMul(x :int, y :int): int
+}
+
+function myMul(x: int, y: int): int
 decreases (if (x <= 0) then -x else x)
-{if (x == 0) then 0 else if (x > 0) then myAdd(myMul(x - 1, y), y) else mySub(y, myMul(x + 1, y))}function mySub(x :int, y :int): int
+{if (x == 0) then 0 else if (x > 0) then myAdd(myMul(x - 1, y), y) else mySub(y, myMul(x + 1, y))}
+
+function mySub(x: int, y: int): int
 decreases (if (y <= 0) then -y else y)
-{if (y == 0) then -x else if (y > 0) then mySub(x - 1, y - 1) else mySub(x + 1, y + 1)}function myAdd(x :int, y :int): int
+{if (y == 0) then -x else if (y > 0) then mySub(x - 1, y - 1) else mySub(x + 1, y + 1)}
+
+function myAdd(x: int, y: int): int
 decreases (if (x <= 0) then -x else x)
-{if (x == 0) then y else if (x > 0) then myAdd(x - 1, y + 1) else myAdd(x + 1, y - 1)}function mul(x :int, y :int): int
+{if (x == 0) then y else if (x > 0) then myAdd(x - 1, y + 1) else myAdd(x + 1, y - 1)}
+
+function mul(x: int, y: int): int
 decreases (if (x <= 0) then -x else x)
-{if (x == 0) then 0 else if (x > 0) then add(mul(x - 1, y), y) else sub(mul(x + 1, y), y)}function sub(x :int, y :int): int
+{if (x == 0) then 0 else if (x > 0) then add(mul(x - 1, y), y) else sub(mul(x + 1, y), y)}
+
+function sub(x: int, y: int): int
 decreases (if (x <= 0) then -x else x)
-{if (x == 0) then -y else if (x > 0) then sub(x - 1, y - 1) else sub(x + 1, y + 1)}function add(x :int, y :int): int
+{if (x == 0) then -y else if (x > 0) then sub(x - 1, y - 1) else sub(x + 1, y + 1)}
+
+function add(x: int, y: int): int
 decreases (if (x <= 0) then -x else x)
-{if (x == 0) then y else if (x > 0) then add(x - 1, y + 1) else add(x + 1, y - 1)}lemma eval1Equivalence(op :OpKind, x :int, y :int)
+{if (x == 0) then y else if (x > 0) then add(x - 1, y + 1) else add(x + 1, y - 1)}
+
+lemma eval1Equivalence(op: OpKind, x: int, y: int)
 ensures evalM(op, x, y) == eval1(op, x, y)
 {{}}
+
