src/test/output/i1264.dfy
@@ -1,31 +1,43 @@
-datatype List<T> = Nil | Cons(head :T, tail :List<T>)
-function replace<T(==)>(l1 :List<T>, x :T, l2 :List<T>): List<T>
+datatype List<T> = Nil | Cons(head: T, tail: List<T>)
+
+function replace<T(==)>(l1: List<T>, x: T, l2: List<T>): List<T>
 decreases (l1)
 {match l1 {
 case Nil() => Nil
 case Cons(y, ys) => if x == y then append(l2, replace(ys, x, l2)) else Cons(y, replace(ys, x, l2))
 }
-}function slowReplace<T(==)>(l1 :List<T>, x :T, l2 :List<T>): List<T>
-{join(split(l1, x), l2)}function join<T>(ll :List<List<T>>, l :List<T>): List<T>
+}
+
+function slowReplace<T(==)>(l1: List<T>, x: T, l2: List<T>): List<T>
+{join(split(l1, x), l2)}
+
+function join<T>(ll: List<List<T>>, l: List<T>): List<T>
 decreases (ll)
 {match ll {
 case Nil => Nil
 case Cons(l1, Nil) => l1
 case Cons(l1, ls) => append(append(l1, l), join(ls, l))
 }
-}function split<T(==)>(l :List<T>, x :T): List<List<T>>
+}
+
+function split<T(==)>(l: List<T>, x: T): List<List<T>>
 decreases (l)
 {match l {
 case Nil => Cons(Nil, Nil)
 case Cons(y, ys) => if (x == y) then Cons(Nil, split(ys, x)) else var r := split(ys, x);
 Cons(Cons(y, r.head), r.tail)
 }
-}function append<T>(l1 :List<T>, l2 :List<T>): List<T>
+}
+
+function append<T>(l1: List<T>, l2: List<T>): List<T>
 decreases (l1)
 {match l1 {
 case Nil() => l2
 case Cons(hd, tl) => Cons(hd, append(tl, l2))
 }
-}lemma slowReplaceEquivalence<T(==)>(l1 :List<T>, x :T, l2 :List<T>)
+}
+
+lemma slowReplaceEquivalence<T(==)>(l1: List<T>, x: T, l2: List<T>)
 ensures replace(l1, x, l2) == slowReplace(l1, x, l2)
 {{}}
+
