src/test/output/inlining.dfy
@@ -1,5 +1,10 @@
-function inlining_1(x :int): int
-{if (x > 0) then inlining_1(x - 1) + 1 else if (x < 0) then 0 else x}function inlining_2(x :int): int
-{if (x > 1) then inlining_2(x - 2) + 2 else if (x < 0) then 0 else x}lemma inlining_2Equivalence(x :int)
+function inlining_1(x: int): int
+{if (x > 0) then inlining_1(x - 1) + 1 else if (x < 0) then 0 else x}
+
+function inlining_2(x: int): int
+{if (x > 1) then inlining_2(x - 2) + 2 else if (x < 0) then 0 else x}
+
+lemma inlining_2Equivalence(x: int)
 ensures inlining_1(x) == inlining_2(x)
 {{}}
+
