src/test/output/iseven1.dfy
@@ -1,13 +1,26 @@
-function isEvenTopLvlM(x :int): bool
-{isEven(x)}function isEvenTopLvl1(x :int): bool
-{myIsEven(x)}function myIsEven(x :int): bool
+function isEvenTopLvlM(x: int): bool
+{isEven(x)}
+
+function isEvenTopLvl1(x: int): bool
+{myIsEven(x)}
+
+function myIsEven(x: int): bool
 decreases (if (x <= 0) then 0 else x)
-{if (x < 0) then false else if (x == 0) then true else !myIsOdd(x - 1)}function myIsOdd(x :int): bool
+{if (x < 0) then false else if (x == 0) then true else !myIsOdd(x - 1)}
+
+function myIsOdd(x: int): bool
 decreases (if (x <= 0) then 0 else x)
-{if (x <= 0) then false else if (x == 1) then true else !myIsEven(x - 1)}function isEven(x :int): bool
+{if (x <= 0) then false else if (x == 1) then true else !myIsEven(x - 1)}
+
+function isEven(x: int): bool
 decreases (if (x <= 0) then 0 else x)
-{if (x < 0) then false else if (x == 0) then true else !isOdd(x - 1)}function isOdd(x :int): bool
+{if (x < 0) then false else if (x == 0) then true else !isOdd(x - 1)}
+
+function isOdd(x: int): bool
 decreases (if (x <= 0) then 0 else x)
-{if (x <= 0) then false else if (x == 1) then true else !isEven(x - 1)}lemma isEvenTopLvl1Equivalence(x :int)
+{if (x <= 0) then false else if (x == 1) then true else !isEven(x - 1)}
+
+lemma isEvenTopLvl1Equivalence(x: int)
 ensures isEvenTopLvlM(x) == isEvenTopLvl1(x)
 {{}}
+
