src/test/output/iseven3.dfy
@@ -1,31 +1,43 @@
-datatype UnaryNat = Zero | Succ(pred :UnaryNat)
-function isEven1(un :UnaryNat): bool
+datatype UnaryNat = Zero | Succ(pred: UnaryNat)
+
+function isEven1(un: UnaryNat): bool
 {match un {
 case Zero => true
 case Succ(pred) => isOdd1(pred)
 }
-}function isEven2(un :UnaryNat): bool
+}
+
+function isEven2(un: UnaryNat): bool
 {match un {
 case Zero => true
 case Succ(pred) => isOdd2(pred)
 }
-}function isOdd2(un :UnaryNat): bool
+}
+
+function isOdd2(un: UnaryNat): bool
 {match un {
 case Zero => false
 case Succ(Zero) => true
 case Succ(Succ(Zero)) => false
 case _ => isEven2(prev(un))
 }
-}function isOdd1(un :UnaryNat): bool
+}
+
+function isOdd1(un: UnaryNat): bool
 {match un {
 case Zero => false
 case Succ(pred) => isEven1(pred)
 }
-}function prev(un :UnaryNat): UnaryNat
+}
+
+function prev(un: UnaryNat): UnaryNat
 {match un {
 case Zero => Zero
 case Succ(n0) => n0
 }
-}lemma isEven2Equivalence(un :UnaryNat)
+}
+
+lemma isEven2Equivalence(un: UnaryNat)
 ensures isEven1(un) == isEven2(un)
 {{}}
+
