src/test/output/limit2.dfy
@@ -1,5 +1,10 @@
-function limit2_1(n :int): int
-{if (n <= 0) then n else n + limit2_1(n - 1)}function limit2_2(n :int): int
-{if (n <= 1) then n else n + limit2_2(n - 1)}lemma limit2_2Equivalence(n :int)
+function limit2_1(n: int): int
+{if (n <= 0) then n else n + limit2_1(n - 1)}
+
+function limit2_2(n: int): int
+{if (n <= 1) then n else n + limit2_2(n - 1)}
+
+lemma limit2_2Equivalence(n: int)
 ensures limit2_1(n) == limit2_2(n)
 {{}}
+
