src/test/output/max.dfy
@@ -1,19 +1,35 @@
-datatype List<T> = Nil | Cons(head :T, tail :List<T>)
-function maxR(l :seq<int>): int
+datatype List<T> = Nil | Cons(head: T, tail: List<T>)
+
+function maxR(l: seq<int>): int
 {if |l| == 0 then -1 else if |l| == 1 then l[0] else var m := maxR(l[1 ..]);
-if l[0] > m then l[0] else m}function maxT(l :seq<int>): int
-{if |l| == 0 then -1 else foldLeft(bigger, l[0], l[1 ..])}function maxC(l :seq<int>): int
+if l[0] > m then l[0] else m}
+
+function maxT(l: seq<int>): int
+{if |l| == 0 then -1 else foldLeft(bigger, l[0], l[1 ..])}
+
+function maxC(l: seq<int>): int
 decreases |l|
-{if |l| == 0 then -1 else if |l| == 1 then l[0] else if l[0] > l[1] then maxC([l[0]] + l[2 ..]) else maxC(l[1 ..])}function bigger(a :int, b :int): int
-{if a >= b then a else b}function foldLeft<T, U>(f :(U, T) -> U, acc :U, l :seq<T>): U
-{if |l| == 0 then acc else foldLeft(f, f(acc, l[0]), l[1 ..])}function length<T>(l :List<T>): nat
+{if |l| == 0 then -1 else if |l| == 1 then l[0] else if l[0] > l[1] then maxC([l[0]] + l[2 ..]) else maxC(l[1 ..])}
+
+function bigger(a: int, b: int): int
+{if a >= b then a else b}
+
+function foldLeft<T, U>(f: (U, T) -> U, acc: U, l: seq<T>): U
+{if |l| == 0 then acc else foldLeft(f, f(acc, l[0]), l[1 ..])}
+
+function length<T>(l: List<T>): nat
 {match l {
 case Nil => 0
 case Cons(_, tl) => 1 + length(tl)
 }
-}lemma maxTEquivalence(l :seq<int>)
+}
+
+lemma maxTEquivalence(l: seq<int>)
 ensures maxR(l) == maxT(l)
-{{}}lemma maxCEquivalence(l :seq<int>)
+{{}}
+
+lemma maxCEquivalence(l: seq<int>)
 decreases |l|
 ensures maxR(l) == maxC(l)
 {{}}
+
