src/test/output/max3.dfy
@@ -1,33 +1,45 @@
-datatype List<T> = Nil | Cons(head :T, tail :List<T>)
-ghost function maxM(lst :List<int>): int
+datatype List<T> = Nil | Cons(head: T, tail: List<T>)
+
+ghost function maxM(lst: List<int>): int
 {match lst {
 case Nil => var x: int :| true;
 x
 case Cons(hd, tl) => foldM((x, y) => if (x > y) then x else y, lst, hd)
 }
-}ghost function max1(lst :List<int>): int
+}
+
+ghost function max1(lst: List<int>): int
 {match lst {
 case Nil => var x: int :| true;
 x
 case Cons(hd, tl) => fold1((x, y) => if (x > y) then x else y, lst, hd)
 }
-}function fold1(f :(int, int) -> int, l :List<int>, a :int): int
+}
+
+function fold1(f: (int, int) -> int, l: List<int>, a: int): int
 decreases (l)
 {match l {
 case Nil => a
 case Cons(hd, tl) => f(hd, fold1(f, tl, a))
 }
-}function norm(l :List<int>, f :int): int
+}
+
+function norm(l: List<int>, f: int): int
 {match l {
 case Nil => -1
 case _ => f
 }
-}function foldM(f :(int, int) -> int, l :List<int>, a :int): int
+}
+
+function foldM(f: (int, int) -> int, l: List<int>, a: int): int
 decreases (l)
 {match l {
 case Nil => a
 case Cons(hd, tl) => f(hd, foldM(f, tl, a))
 }
-}lemma max1Equivalence(lst :List<int>)
+}
+
+lemma max1Equivalence(lst: List<int>)
 ensures maxM(lst) == max1(lst)
 {{}}
+
