src/test/output/separate.dfy
@@ -1,6 +1,8 @@
-datatype Animal = Sheep(id :int) | Goat(id :int)
-datatype List<T> = Nil | Cons(head :T, tail :List<T>)
-function separateM(xs :List<Animal>): (List<Animal>, List<Animal>)
+datatype Animal = Sheep(id: int) | Goat(id: int)
+
+datatype List<T> = Nil | Cons(head: T, tail: List<T>)
+
+function separateM(xs: List<Animal>): (List<Animal>, List<Animal>)
 {match xs {
 case Nil => (Nil, Nil)
 case Cons(Sheep(id), t) => var (s2, g2) := separateM(t);
@@ -8,7 +10,9 @@ case Cons(Sheep(id), t) => var (s2, g2) := separateM(t);
 case Cons(Goat(id), t) => var (s2, g2) := separateM(t);
 (s2, Cons(Goat(id), g2))
 }
-}function separate2(xs :List<Animal>): (List<Animal>, List<Animal>)
+}
+
+function separate2(xs: List<Animal>): (List<Animal>, List<Animal>)
 {match xs {
 case Nil => (Nil, Nil)
 case Cons(Sheep(id), t) => var (s2, g2) := separate2(t);
@@ -16,7 +20,9 @@ case Cons(Sheep(id), t) => var (s2, g2) := separate2(t);
 case Cons(Goat(id), t) => var (s2, g2) := separate2(t);
 (s2, g2)
 }
-}function separate1(xs :List<Animal>): (List<Animal>, List<Animal>)
+}
+
+function separate1(xs: List<Animal>): (List<Animal>, List<Animal>)
 {match xs {
 case Nil => (Nil, Nil)
 case Cons(Sheep(id), t) => var (s2, g2) := separate1(t);
@@ -24,8 +30,13 @@ case Cons(Sheep(id), t) => var (s2, g2) := separate1(t);
 case Cons(Goat(id), t) => var (s2, g2) := separate1(t);
 (s2, Cons(Goat(id), g2))
 }
-}lemma separate2Equivalence(xs :List<Animal>)
+}
+
+lemma separate2Equivalence(xs: List<Animal>)
 ensures separateM(xs) == separate2(xs)
-{{}}lemma separate1Equivalence(xs :List<Animal>)
+{{}}
+
+lemma separate1Equivalence(xs: List<Animal>)
 ensures separateM(xs) == separate1(xs)
 {{}}
+
