src/test/output/sortedArray.dfy
@@ -1,12 +1,19 @@
-function isSortedArrayM(a :seq<int>, start :int, n :int): bool
+function isSortedArrayM(a: seq<int>, start: int, n: int): bool
 decreases (n)
 requires (0 <= start && n >= start && n <= |a|)
-{if n <= succM(start) then true else if a[n - 2] > a[n - 1] then false else isSortedArrayM(a, start, n - 1)}function isSortedArray(a :seq<int>, start :int, n :int): bool
+{if n <= succM(start) then true else if a[n - 2] > a[n - 1] then false else isSortedArrayM(a, start, n - 1)}
+
+function isSortedArray(a: seq<int>, start: int, n: int): bool
 decreases (n)
 requires (0 <= start && n >= start && n <= |a|)
-{if n == start then true else if n == start + 1 then true else if a[n - 2] > a[n - 1] then false else isSortedArray(a, start, n - 1)}function succM(n :int): int
-{n + 1}lemma isSortedArrayEquivalence(a :seq<int>, start :int, n :int)
+{if n == start then true else if n == start + 1 then true else if a[n - 2] > a[n - 1] then false else isSortedArray(a, start, n - 1)}
+
+function succM(n: int): int
+{n + 1}
+
+lemma isSortedArrayEquivalence(a: seq<int>, start: int, n: int)
 decreases (n)
 requires (0 <= start && n >= start && n <= |a|)
 ensures isSortedArrayM(a, start, n) == isSortedArray(a, start, n)
 {{}}
+
