src/test/output/sum.dfy
@@ -1,5 +1,10 @@
-function sum1(n :int): int
-{if (n <= 1) then n else n + n - 1 + sum1(n - 2)}function sum2(n :int): int
-{if (n <= 1) then n else n + sum2(n - 1)}lemma sum2Equivalence(n :int)
+function sum1(n: int): int
+{if (n <= 1) then n else n + n - 1 + sum1(n - 2)}
+
+function sum2(n: int): int
+{if (n <= 1) then n else n + sum2(n - 1)}
+
+lemma sum2Equivalence(n: int)
 ensures sum1(n) == sum2(n)
 {{}}
+
