src/test/output/unfoldingSorted.dfy
@@ -1,23 +1,39 @@
-datatype Option<T> = None | Some(value :T)
-datatype List<T> = Nil | Cons(head :T, tail :List<T>)
-function unfoldingSortedM<S, T>(start :S, next :S -> Option<(S, T)>, leq :(T, T) -> bool, max :int): List<T>
-{loopM(start, next, leq, max, Nil)}function unfoldingSorted5<State, Elem>(start :State, next :State -> Option<(State, Elem)>, leq :(Elem, Elem) -> bool, max :int): List<Elem>
-{go5(start, next, leq, Nil, max)}function unfoldingSorted4<State, Elem>(start :State, next :State -> Option<(State, Elem)>, leq :(Elem, Elem) -> bool, max :int): List<Elem>
-{go4(start, next, leq, Nil, max)}function unfoldingSorted3<State, Elem>(start :State, next :State -> Option<(State, Elem)>, leq :(Elem, Elem) -> bool, max :int): List<Elem>
-{go3(start, next, Nil, max)}function unfoldingSorted1<State, Elem>(start :State, next :State -> Option<(State, Elem)>, leq :(Elem, Elem) -> bool, max :int): List<Elem>
-{go1(start, next, leq, Nil, max)}function go5<State, Elem>(s :State, next :State -> Option<(State, Elem)>, leq :(Elem, Elem) -> bool, xs :List<Elem>, fuel :int): List<Elem>
+datatype Option<T> = None | Some(value: T)
+
+datatype List<T> = Nil | Cons(head: T, tail: List<T>)
+
+function unfoldingSortedM<S, T>(start: S, next: S -> Option<(S, T)>, leq: (T, T) -> bool, max: int): List<T>
+{loopM(start, next, leq, max, Nil)}
+
+function unfoldingSorted5<State, Elem>(start: State, next: State -> Option<(State, Elem)>, leq: (Elem, Elem) -> bool, max: int): List<Elem>
+{go5(start, next, leq, Nil, max)}
+
+function unfoldingSorted4<State, Elem>(start: State, next: State -> Option<(State, Elem)>, leq: (Elem, Elem) -> bool, max: int): List<Elem>
+{go4(start, next, leq, Nil, max)}
+
+function unfoldingSorted3<State, Elem>(start: State, next: State -> Option<(State, Elem)>, leq: (Elem, Elem) -> bool, max: int): List<Elem>
+{go3(start, next, Nil, max)}
+
+function unfoldingSorted1<State, Elem>(start: State, next: State -> Option<(State, Elem)>, leq: (Elem, Elem) -> bool, max: int): List<Elem>
+{go1(start, next, leq, Nil, max)}
+
+function go5<State, Elem>(s: State, next: State -> Option<(State, Elem)>, leq: (Elem, Elem) -> bool, xs: List<Elem>, fuel: int): List<Elem>
 decreases (if (fuel <= 0) then 0 else fuel)
 {if (fuel <= 0) then xs else match next(s) {
 case Some((nxtS, t)) => go5(nxtS, next, leq, insertSorted5(t, leq, xs), fuel - 1)
 case None => xs
 }
-}function insertSorted5<Elem>(t :Elem, leq :(Elem, Elem) -> bool, xs :List<Elem>): List<Elem>
+}
+
+function insertSorted5<Elem>(t: Elem, leq: (Elem, Elem) -> bool, xs: List<Elem>): List<Elem>
 decreases (xs)
 {match xs {
 case Nil => Cons(t, Nil)
 case Cons(hd, tl) => if (leq(t, hd)) then Cons(t, xs) else Cons(hd, insertSorted5(t, leq, tl))
 }
-}function go4<State, Elem>(s :State, next :State -> Option<(State, Elem)>, leq :(Elem, Elem) -> bool, xs :List<Elem>, fuel :int): List<Elem>
+}
+
+function go4<State, Elem>(s: State, next: State -> Option<(State, Elem)>, leq: (Elem, Elem) -> bool, xs: List<Elem>, fuel: int): List<Elem>
 decreases (if (fuel <= 0) then 0 else fuel)
 {if (fuel <= 0) then xs else match next(s) {
 case Some((nxtS, t)) => go4(nxtS, next, leq, insertSorted4(t, leq, xs), fuel - 1)
@@ -27,54 +43,77 @@ case Nil => xs
 }
 
 }
-}function insertSorted4<Elem>(t :Elem, leq :(Elem, Elem) -> bool, xs :List<Elem>): List<Elem>
+}
+
+function insertSorted4<Elem>(t: Elem, leq: (Elem, Elem) -> bool, xs: List<Elem>): List<Elem>
 decreases (xs)
 {match xs {
 case Nil => Cons(t, Nil)
 case Cons(hd, tl) => if (leq(t, hd)) then Cons(t, xs) else Cons(hd, insertSorted4(t, leq, tl))
 }
-}function go3<State, Elem>(s :State, next :State -> Option<(State, Elem)>, xs :List<Elem>, fuel :int): List<Elem>
+}
+
+function go3<State, Elem>(s: State, next: State -> Option<(State, Elem)>, xs: List<Elem>, fuel: int): List<Elem>
 decreases (if (fuel <= 0) then 0 else fuel)
 {if (fuel <= 0) then xs else match next(s) {
 case Some((nxtS, t)) => go3(nxtS, next, insertSorted3(t, xs), fuel - 1)
 case None => xs
 }
-}function insertSorted3<Elem>(t :Elem, xs :List<Elem>): List<Elem>
+}
+
+function insertSorted3<Elem>(t: Elem, xs: List<Elem>): List<Elem>
 decreases (xs)
 {match xs {
 case Nil => Cons(t, Nil)
 case Cons(hd, tl) => Cons(hd, insertSorted3(t, tl))
 }
-}function go1<State, Elem>(s :State, next :State -> Option<(State, Elem)>, leq :(Elem, Elem) -> bool, xs :List<Elem>, fuel :int): List<Elem>
+}
+
+function go1<State, Elem>(s: State, next: State -> Option<(State, Elem)>, leq: (Elem, Elem) -> bool, xs: List<Elem>, fuel: int): List<Elem>
 decreases (if (fuel <= 0) then 0 else fuel)
 {if (fuel <= 0) then xs else match next(s) {
 case Some((nxtS, t)) => go1(nxtS, next, leq, insertSorted1(t, leq, xs), fuel - 1)
 case None => xs
 }
-}function insertSorted1<Elem>(t :Elem, leq :(Elem, Elem) -> bool, xs :List<Elem>): List<Elem>
+}
+
+function insertSorted1<Elem>(t: Elem, leq: (Elem, Elem) -> bool, xs: List<Elem>): List<Elem>
 decreases (xs)
 {match xs {
 case Nil => Cons(t, Nil)
 case Cons(hd, tl) => if (leq(t, hd)) then Cons(t, xs) else Cons(hd, insertSorted1(t, leq, tl))
 }
-}function loopM<S, T>(s :S, next :S -> Option<(S, T)>, leq :(T, T) -> bool, fuel :int, xs :List<T>): List<T>
+}
+
+function loopM<S, T>(s: S, next: S -> Option<(S, T)>, leq: (T, T) -> bool, fuel: int, xs: List<T>): List<T>
 decreases (if (fuel <= 0) then 0 else fuel)
 {if (fuel <= 0) then xs else match next(s) {
 case Some((nxtS, t)) => loopM(nxtS, next, leq, fuel - 1, insertM(xs, leq, t))
 case None => xs
 }
-}function insertM<T>(xs :List<T>, leq :(T, T) -> bool, t :T): List<T>
+}
+
+function insertM<T>(xs: List<T>, leq: (T, T) -> bool, t: T): List<T>
 decreases (xs)
 {match xs {
 case Nil => Cons(t, Nil)
 case Cons(hd, tl) => if (leq(t, hd)) then Cons(t, xs) else Cons(hd, insertM(tl, leq, t))
 }
-}lemma unfoldingSorted5Equivalence<State, Elem>(start :State, next :State -> Option<(State, Elem)>, leq :(Elem, Elem) -> bool, max :int)
+}
+
+lemma unfoldingSorted5Equivalence<State, Elem>(start: State, next: State -> Option<(State, Elem)>, leq: (Elem, Elem) -> bool, max: int)
 ensures unfoldingSortedM(start, next, leq, max) == unfoldingSorted5(start, next, leq, max)
-{{}}lemma unfoldingSorted4Equivalence<State, Elem>(start :State, next :State -> Option<(State, Elem)>, leq :(Elem, Elem) -> bool, max :int)
+{{}}
+
+lemma unfoldingSorted4Equivalence<State, Elem>(start: State, next: State -> Option<(State, Elem)>, leq: (Elem, Elem) -> bool, max: int)
 ensures unfoldingSortedM(start, next, leq, max) == unfoldingSorted4(start, next, leq, max)
-{{}}lemma unfoldingSorted3Equivalence<State, Elem>(start :State, next :State -> Option<(State, Elem)>, leq :(Elem, Elem) -> bool, max :int)
+{{}}
+
+lemma unfoldingSorted3Equivalence<State, Elem>(start: State, next: State -> Option<(State, Elem)>, leq: (Elem, Elem) -> bool, max: int)
 ensures unfoldingSortedM(start, next, leq, max) == unfoldingSorted3(start, next, leq, max)
-{{}}lemma unfoldingSorted1Equivalence<State, Elem>(start :State, next :State -> Option<(State, Elem)>, leq :(Elem, Elem) -> bool, max :int)
+{{}}
+
+lemma unfoldingSorted1Equivalence<State, Elem>(start: State, next: State -> Option<(State, Elem)>, leq: (Elem, Elem) -> bool, max: int)
 ensures unfoldingSortedM(start, next, leq, max) == unfoldingSorted1(start, next, leq, max)
 {{}}
+
