src/test/output/unique.dfy
@@ -1,32 +1,48 @@
-datatype List<T> = Nil | Cons(head :T, tail :List<T>)
-function uniqR(lst :List<int>): List<int>
-{unique(lst, Nil)}function uniqA(lst :List<int>): List<int>
-{distinct(Nil, lst)}function distinct(a :List<int>, b :List<int>): List<int>
+datatype List<T> = Nil | Cons(head: T, tail: List<T>)
+
+function uniqR(lst: List<int>): List<int>
+{unique(lst, Nil)}
+
+function uniqA(lst: List<int>): List<int>
+{distinct(Nil, lst)}
+
+function distinct(a: List<int>, b: List<int>): List<int>
 decreases b
 {match b {
 case Nil => a
 case Cons(hd, tl) => if isin(hd, a) then distinct(a, tl) else distinct(append(a, Cons(hd, Nil)), tl)
 }
-}function isin(a :int, lst :List<int>): bool
+}
+
+function isin(a: int, lst: List<int>): bool
 {match lst {
 case Nil => false
 case Cons(hd, tl) => a == hd || isin(a, tl)
 }
-}function unique(l :List<int>, r :List<int>): List<int>
+}
+
+function unique(l: List<int>, r: List<int>): List<int>
 {match l {
 case Nil => r
 case Cons(hd, tl) => if !find(r, hd) then unique(tl, append(r, Cons(hd, Nil))) else unique(tl, r)
 }
-}function find(lst :List<int>, n :int): bool
+}
+
+function find(lst: List<int>, n: int): bool
 {match lst {
 case Nil => false
 case Cons(hd, tl) => n == hd || find(tl, n)
 }
-}function append(l1 :List<int>, l2 :List<int>): List<int>
+}
+
+function append(l1: List<int>, l2: List<int>): List<int>
 {match l1 {
 case Nil => l2
 case Cons(hd, tl) => Cons(hd, append(tl, l2))
 }
-}lemma uniqAEquivalence(lst :List<int>)
+}
+
+lemma uniqAEquivalence(lst: List<int>)
 ensures uniqR(lst) == uniqA(lst)
 {{}}
+
