src/test/output/unrolling.dfy
@@ -1,5 +1,10 @@
-function fact13_1(n :int): int
-{if (n <= 1) then 1 else if (n == 2) then 2 else if (n == 3) then 6 else if (n == 4) then 24 else n * (n - 1) * (n - 2) * (n - 3) * fact13_1(n - 4)}function fact13_2(n :int): int
-{if (n <= 1) then 1 else if (n == 2) then 2 else if (n == 3) then 6 else if (n == 4) then 24 else if (n == 5) then 120 else if (n == 6) then 720 else if (n == 7) then 5040 else if (n == 8) then 40320 else n * (n - 1) * (n - 2) * (n - 3) * fact13_2(n - 4)}lemma fact13_2Equivalence(n :int)
+function fact13_1(n: int): int
+{if (n <= 1) then 1 else if (n == 2) then 2 else if (n == 3) then 6 else if (n == 4) then 24 else n * (n - 1) * (n - 2) * (n - 3) * fact13_1(n - 4)}
+
+function fact13_2(n: int): int
+{if (n <= 1) then 1 else if (n == 2) then 2 else if (n == 3) then 6 else if (n == 4) then 24 else if (n == 5) then 120 else if (n == 6) then 720 else if (n == 7) then 5040 else if (n == 8) then 40320 else n * (n - 1) * (n - 2) * (n - 3) * fact13_2(n - 4)}
+
+lemma fact13_2Equivalence(n: int)
 ensures fact13_1(n) == fact13_2(n)
 {{}}
+
